test/lean/Proofs.lean
@@ -4,13 +4,41 @@ open Primitives
 open Result
 open test
 
--- @[pspec] -- the [pspec] attribute saves the theorem in a database, for [progress] to use it
--- theorem mul2_add1_spec (x : U32) (h : 2 * ↑x + 1 ≤ U32.max)
---   : ∃ y, functions.mul2_add1 x = ret y ∧
---   ↑ y = 2 * ↑x + (1 : Int)
---   := by
---   rw [functions.mul2_add1]
---   -- progress with U32.add_spec as ⟨ x1 ⟩
---   progress as ⟨ x1 .. ⟩ -- [progress] automatically lookups [U32.add_spec]
---   progress as ⟨ x2 .. ⟩ -- same
---   simp at *; scalar_tac
+namespace test
+
+namespace arithmetics
+
+def BigInt.valImpl (l : List U64) : Int :=
+  match l with
+  | a::b => a.val + (valImpl b) * (2 ^ 64)
+  | [] => 0
+
+def BigInt.val {N : Usize} (x : BigInt N) : Int := valImpl x.num.val
+
+def BigInt.max_value (N : Usize) : Int := (U64.max + 1) ^ (Int.toNat N.val) - 1
+
+theorem adc_for_add_with_carry_spec (a : U64) (b : U64) (carry : U8) :
+  match adc_for_add_with_carry a b carry with
+  | ret new_carry => new_carry = (a.val + b.val + carry.val) / (2 ^ 64)
+  | _ => ⊥
+  := by sorry
+
+theorem adc_for_add_with_carry_back_spec (a : U64) (b : U64) (carry : U8) :
+  ∃ new_a, adc_for_add_with_carry_back a b carry = .ret new_a ∧
+  new_a = (a.val + b.val + carry.val) * 2 ^ 64 := by sorry
+
+
+lemma add_with_carry_overflow : 
+  ∀ (N : Usize) (self : arithmetics.BigInt N) (other : arithmetics.BigInt N),
+  ∃ b, arithmetics.BigInt.add_with_carry N self other = .ret b ∧
+  ¬b ↔ self.val + other.val ≤ BigInt.max_value N := sorry
+    -- by unfold arithmetics.BigInt.add_with_carry
+
+lemma add_with_carry_correct :
+  ∀ (N : Usize) (self : arithmetics.BigInt N) (other : arithmetics.BigInt N),
+  ∃ v, arithmetics.BigInt.add_with_carry_back N self other = .ret v ∧
+  v.val = (self.val + other.val) % (BigInt.max_value N) := sorry
+
+end arithmetics
+
+end test
