Dockerfile
@@ -17,19 +17,20 @@ ENV LANG='en_US.UTF-8' LANGUAGE='en_US:en' LC_ALL='en_US.UTF-8'
 ENV USER=root
 RUN echo "source $HOME/.nix-profile/etc/profile.d/nix.sh" >> "$HOME/.bashrc"
 
+# Install Rust
+RUN curl --proto '=https' --tlsv1.2 -sSf https://sh.rustup.rs | sh -s -- -y
+ENV PATH=/root/.cargo/bin:$PATH
+
 # Build charon and aeneas
 RUN git clone https://github.com/AeneasVerif/charon.git 
-RUN . "$HOME/.nix-profile/etc/profile.d/nix.sh" && cd charon && nix build .#charon -o nix-build --extra-experimental-features nix-command --extra-experimental-features flakes && make build-charon-rust && cd ..
+RUN . "$HOME/.nix-profile/etc/profile.d/nix.sh" && cd charon && nix build .#charon -o nix-build --extra-experimental-features nix-command --extra-experimental-features flakes && cd ..
+RUN cd charon && make build-charon-rust && cd ..
 RUN git clone https://github.com/AeneasVerif/aeneas.git 
 RUN . "$HOME/.nix-profile/etc/profile.d/nix.sh" && cd aeneas && nix build .#aeneas -o nix-build --extra-experimental-features nix-command --extra-experimental-features flakes && cd ..
 
 # Setup charon and aeneas
-ENV PATH="/charon//bin:${PATH}"
+ENV PATH="/charon/bin:${PATH}"
 ENV PATH="/aeneas/nix-build/bin:${PATH}"
-
-# Install Rust
-RUN curl --proto '=https' --tlsv1.2 -sSf https://sh.rustup.rs | sh -s -- -y
-ENV PATH=/root/.cargo/bin:$PATH
 
 # Install Lean
 RUN curl https://raw.githubusercontent.com/leanprover/elan/master/elan-init.sh -sSf | sh -s -- -y
